\section{Commutators and  Uncertainty Principle}
For a Hermitian operator $A$, we define the variance $\Delta A$ using
the expression (expectation of square minus square of expectation)
\begin{equation*}
  \begin{split}
    (\Delta A)^2 & =  \expval{A^2} - \expval{A}^2 \\
                 & =  \expval{(A-\expval{A})^2} \\
                 & =  \expval{U^2}.
  \end{split}
\end{equation*}
where $U = A-\expval{A}$. We will have a similar definition for
another Hermitian operator $B$. For this operator, we will define
another operator $V$ so that the following relationships hold
\begin{equation*}
  \begin{split}
    U & = A - \expval{A} \\
    V & = B - \expval{B} \\
    (\Delta A)^2 & = \expval{U^2} \\
    (\Delta B)^2 & = \expval{V^2}.
  \end{split}
\end{equation*}

Now consider the expression $\expval{U + i\lambda V}$ for some
arbitrary but real $\lambda$. The following relationships hold.
\begin{equation}\label{ineq1}
\begin{split}
  \expval{U + i\lambda V} & \ge 0 \\
  \expval{U} + \lambda^2\expval{V} +
  i\lambda\expval{U\cdot V} - i\lambda\expval{V\cdot U} &
  \ge 0. 
\end{split}
\end{equation}

If we define the commutator of $U$ and $V$ as
\[
\commutator{U}{V} = UV - VU,
\]
then note that $\commutator{U}{V} = \commutator{A}{B}$. Then
Eqn~\ref{ineq1} can be simplified as
\begin{equation*}
  \expval{U} + \lambda^2\expval{V} + i\lambda\expval{\commutator{U}{V}} \ge 0.
\end{equation*}

This is a quadratic equation in $\lambda$ which cannot have a real
solution implying that the discriminant is negative. This implies
\begin{equation*}
  \begin{split}
    -\expval{\commutator{U}{V}}^2 -4\expval{U}\expval{V} & \le 0 \\
    4\expval{U}\expval{V} & \ge -\expval{\commutator{U}{V}}^2 \\
    (\Delta A)^2(\Delta B)^2 \ge \expval{\frac{i}{2}\commutator{U}{V}}
    \\
    (\Delta A)(\Delta B) \ge \frac{i}{2}\expval{\commutator{A}{B}}
  \end{split}
\end{equation*}

This is the general uncertainty relation between observables.
